\label{parsing}
\section{Parsing}
\subsection{LL(1) Grammar}
 This grammar is not LL(1) because it has a rule with left recursion: $B:=Bv$ and $B:=w$.\\
\subsection{Modify the grammar}
We replaced the left recursion with a right recursion to avoid the problem indicated in the first exercise.
\begin{center}            
	$B:=wB'$\\
        $B':=vB'$\\
        $B':=\epsilon$\\
\end{center}
Thus, we removed from the grammar the rules $B:=Bv$ and $B:=w$ and we introduced rules above.\\
\subsection{Sets for this grammar}
$first(u) = \{u\}\\
            first(v) = \{v\}\\
            first(w) = \{w\}\\
            first(x) = \{x\}\\
            first(y) = \{y\}\\
            first(z) = \{z\}$
                
            $\epsilon \in first(E), first(F), first(B')$

            Rule 1:$ S:== uBDz\\
            first(uBDz) = \{u\}\\
            \rightarrow u \in first(S)$
            
            Rule 2: $B::=wB'\\
            first(wB')=\{w\}\\
            \rightarrow w\in first(B)$
            
            Rule 3: $B'::= wB'\\
            first(vB') = \{v\}\\
            \rightarrow v \in first(B')$
            
            Rule 5: $D::= EF$\\
            $first(EF) = first(E) \backslash \{\epsilon\} \cup first(F)$ (car $E\in first(E)$)$=\{x,y,E\}$\\
            $\rightarrow {x,y,E} \subset first(D)$
            
            Rule 6: $E::= y\\
            y \in first(E)$
            
            Rule 8: $F::=x\\
            x \in first(F)$
            
            $first(S) = \{u\}\\
            first(B) = \{w\}\\
            first(B') = \{v,\epsilon\}\\
            first(D) = \{x,y,\epsilon\}\\
            first(E) = \{y,\epsilon\}\\
            first(F) = \{x, \epsilon\}$
            
            \textbf{Follow}
            
            $\#E \, follow(S)$
            
            Rule 1: $S::= uBDz\\
            \rightarrow \{x,y,z\} \subset B follow(B)\\
            and \, z \in follow(D)$
            
            Rule 2: $\, B::= wB'\\
            \rightarrow follow(B)=\{x,y,z\} \subset follow(B')$
            
            Rule 5: $D::=EF\\
            \rightarrow x \in follow(E)\\
            follow(D) = \{z\} \subset follow(E)\\
            and \, follow(D) = \{z\} \subset follow(F)$
             
            $follow(S) = \{\#\}\\
            follow(B) = \{x,y,z\}\\
            follow(B') = \{x,y,z\}\\
            follow(D) = \{z\}\\
            follow(E) = \{x,z\}\\
            follow(F) = \{z\}$
\subsection{}
          Rule 1: $S::= uBDz\\
            \rightarrow table[S,u] = 1$
            
          Rule 2: $B::= wB'\\
            \rightarrow table[B,w] = 2$
            
          Rule 3: $B'::= vB'\\
            \rightarrow table[B',v] = 3$
            
          Rule 4: $B'::= \epsilon\\
            \rightarrow table[B',x] = 4\\
            \rightarrow table[B',y] = 4\\
            \rightarrow table[B',z] = 4$
            
          Rule 5: $D::= EF\\
            \rightarrow table[D,x] = 5\\
            \rightarrow table[D,y] = 5\\
            \rightarrow table[D,z] = 5$
            
          Rule 6: $E::= y\\
            \rightarrow table[E,y] = 6$
            
          Rule 7: $E::= \epsilon\\
            \rightarrow table[E,x] = 7\\
            \rightarrow talbe[E,z] = 7$
            
          Rule 8: $F::= x\\
            \rightarrow table[F,x] = 8$
            
          Rule 9: $F::= \epsilon\\
            \rightarrow table[F,z] = 9$
            
            \begin{tabular}{ p{2cm} | p{2cm} | p{2cm} | p{2cm} | p{2cm} | p{2cm} | p{2cm}}
                \hline
                & u & v & w & x & y & z \\ \hline                        
                S & 1 & & & & & \\ \hline
                B & & & 2 & & & \\ \hline
                B' & & 3 & & 4 & 4 & 4 \\ \hline
                D & & & & 5 & 5 & 5 \\ \hline
                E & & & & 7 & 6 & 7 \\ \hline
                F & & & & 8 & & 9 \\
                \hline
            \end{tabular}
  

